Finish most of the weak normalization proof

wn.v
@@ -1,15 +1,19 @@
 From Hammer Require Import Tactics Hammer.
 From WR Require Import typing.
-From Coq Require Import ssreflect ssrfun ssrbool Relations.Relation_Operators Logic.PropExtensionality.
+From Coq Require Import ssreflect ssrfun ssrbool.
+From stdpp Require Import relations (rtc(..)).
 
-Set Implicit Arguments.
-Unset Strict Implicit.
-Unset Printing Implicit Defensive.
-
-Fixpoint Interp (b : tm 0) (A : ty) : Prop :=
-  match A with
-  | I => False
-  | Fun A B => forall a, Interp a A -> Interp (App b a) B
+Fixpoint ne {n} (a : tm n) :=
+  match a with
+  | var_tm _ => true
+  | App a b => ne a && nf b
+  | Lam _ _ => false
+  end
+with nf {n} (a : tm n) :=
+  match a with
+  | var_tm _ => true
+  | App a b => ne a && nf b
+  | Lam _ _ => true
   end.
 
 Inductive Red {n} : tm n -> tm n -> Prop :=
@@ -25,152 +29,121 @@ Inductive Red {n} : tm n -> tm n -> Prop :=
 | S_Abs A a b :
   Red (Lam A a) (Lam A b).
 
-#[export]Hint Constructors Red : core.
+#[export]Hint Constructors Red : red.
 
-Lemma Interp_back_preservation A (a b : tm 0) (h : Red a b) : Interp b A -> Interp a A.
+Definition Reds {n} := rtc (@Red n).
+
+Definition wn {n} (a : tm n) := exists b, Reds a b /\ nf b.
+
+Fixpoint Interp n (b : tm n) (A : ty) : Prop :=
+  match A with
+  | I => wn b
+  | Fun A B => forall m (ξ : fin n -> fin m) (a : tm m),
+      Interp m a A -> Interp m (App (ren_tm ξ b) a) B
+  end.
+
+Lemma S_β' {n} a (b t : tm n) A :
+  t = subst_tm (b..) a ->
+  (* ---------------------- *)
+  Red (App (Lam A a) b) t.
+Proof. move=>->. apply S_β. Qed.
+
+Lemma Red_renaming n (a b : tm n) (h : Red a b) m (ξ : fin n -> fin m) :
+  Red (ren_tm ξ a) (ren_tm ξ b).
 Proof.
-  elim : A a b h;
-    hauto q:on inv:Red ctrs:Red.
+  move : m ξ.
+  elim : a b /h =>/=; eauto with red.
+  move => *.
+  apply S_β'. by asimpl.
 Qed.
 
-Definition γ_ok {n} (γ : fin n -> tm 0) (Γ : fin n -> ty) :=
-  forall i, Interp (γ i) (Γ i).
+Lemma Reds_renaming n (a b : tm n) (h : Reds a b) m (ξ : fin n -> fin m) :
+  Reds (ren_tm ξ a) (ren_tm ξ b).
+Proof. elim : h; hauto lq:on ctrs:rtc use:Red_renaming. Qed.
 
-Lemma γ_ok_cons {n} {γ : fin n -> tm 0} {Γ a A} :
-  Interp a A ->
+Lemma ne_nf_renaming n (a : tm n) :
+  forall m (ξ : fin n -> fin m),
+    (ne a -> ne (ren_tm ξ a)) /\ (nf a -> nf (ren_tm ξ a)).
+Proof.
+  elim : n / a; auto.
+  hauto b:on.
+Qed.
+
+Lemma Interp_renaming n A (a : tm n) (h : Interp n a A) :
+  forall m (ξ : fin n -> fin m),
+    Interp m (ren_tm ξ a) A.
+Proof.
+  case : A a h.
+  - move => /= A B a ha m ξ /= p ξ1 b hb.
+    asimpl. by apply ha.
+  - move => /= a h m ξ.
+    case : h => a' [hred ha].
+    exists (ren_tm ξ a').
+    split.
+    + auto using Reds_renaming.
+    + hauto lq:on use:ne_nf_renaming.
+Qed.
+
+Lemma Interp_back_preservation n A (a b : tm n) (h : Red a b) : Interp n b A -> Interp n a A.
+Proof.
+  elim : A n a b h.
+  - hauto lq:on ctrs:Red use:Red_renaming.
+  - hauto q:on ctrs:rtc.
+Qed.
+
+Definition γ_ok {n m} (γ : fin n -> tm m) (Γ : fin n -> ty) :=
+  forall i, Interp m (γ i) (Γ i).
+
+Lemma γ_ok_cons n m {γ : fin n -> tm m} Γ a A :
+  Interp m a A ->
   γ_ok γ Γ ->
   γ_ok (a .: γ) (A .: Γ).
 Proof. hauto q:on inv:option unfold:γ_ok. Qed.
 
-#[export]Hint Resolve γ_ok_cons Interp_back_preservation : core.
+#[export]Hint Resolve γ_ok_cons Interp_back_preservation : semwt.
 
 Definition SemWt {n} (Γ : context n) a A : Prop :=
-  forall γ, γ_ok γ Γ -> Interp (subst_tm γ a) A.
+  forall m (γ : fin n -> tm m), γ_ok γ Γ -> Interp m (subst_tm γ a) A.
 
 Lemma fundamental_lemma {n} (Γ : context n) a A (h : Wt Γ a A) :
   SemWt Γ a A.
 Proof.
   elim : n Γ a A /h; rewrite /SemWt.
   - sfirstorder.
-  - move => n Γ A a B h ih γ hγ /= b hb.
-    apply : Interp_back_preservation; auto.
+  - move => n Γ A a B h ih m γ hγ /= p ξ b hb.
+    apply : Interp_back_preservation; first by apply S_β.
     asimpl.
-    eauto.
-  - sfirstorder.
+    apply ih.
+    apply γ_ok_cons; auto.
+    rewrite /γ_ok => i.
+    renamify.
+    by apply Interp_renaming.
+  - move => /= n Γ a A B b _ iha _ ihb m γ hγ.
+    replace (subst_tm γ a) with (ren_tm id (subst_tm γ a)).
+    + by eauto.
+    + by asimpl.
 Qed.
 
-Definition Prod (PA : tm 0 -> Prop) (PB : tm 0 -> Prop) (b : tm 0) :=
-  forall a, PA a -> PB (App b a).
-
-Inductive Interp_rel : ty -> (tm 0 -> Prop) -> Prop :=
-| Interp_I : Interp_rel I (fun _ => False)
-| Interp_Fun A PA B (PB : tm 0 -> Prop) :
-  Interp_rel A PA ->
-  (forall a, PA a -> Interp_rel B PB) ->
-  Interp_rel (Fun A B) (Prod PA PB).
-
-Lemma Interp_rel_back_preservation A : forall PA (a b : tm 0) (h : Red a b),
-  Interp_rel A PA ->
-  PA b ->
-  PA a.
+Lemma ext_wn n (a : tm n) i :
+    wn (App a (var_tm i)) ->
+    wn a.
 Proof.
-  elim : A.
-  - move => A ihA B ihB PA a b h h1 h2.
-    inversion h1; subst.
-    rewrite /Prod.
-    move => b0 hb0.
-    rewrite /Prod in h2.
-    apply : ihB; eauto.
-  - hauto lq:on inv:Interp_rel.
+  rewrite /wn.
+  case => b0.
+  move E : (App a (var_tm i)) => a0 [h0 h1].
+  move : a i E h1.
+  elim : a0 b0 / h0.
+  - move => ? a i <- /=  /andP.
+    case => *.
+    hauto lq:on ctrs:rtc inv:tm.
+  - hauto lq:on rew:off ctrs:rtc inv:Red.
 Qed.
 
-Definition Interp' (a : tm 0) (A : ty) : Prop :=
-  exists PA, Interp_rel A PA /\ PA a.
+(* Need anti renaming for nf and ne *)
 
-#[export]Hint Unfold Interp' : core.
-
-Lemma Interp_back_preservation' A (a b : tm 0) (h : Red a b) : Interp' b A -> Interp' a A.
+Lemma adequacy n (a : tm n) (A : ty) (h : Interp n a A) :
+  wn a.
 Proof.
-  sfirstorder use:Interp_rel_back_preservation unfold:Interp'.
-Qed.
-
-Definition γ_ok' {n} (γ : fin n -> tm 0) (Γ : fin n -> ty) :=
-  forall i, exists PA, Interp_rel (Γ i) PA /\ PA (γ i).
-
-Lemma γ_ok_cons' {n} {γ : fin n -> tm 0} {Γ a A PA} :
-  Interp_rel A PA ->
-  PA a ->
-  γ_ok' γ Γ ->
-  γ_ok' (a .: γ) (A .: Γ).
-Proof. hauto q:on inv:option unfold:γ_ok'. Qed.
-
-#[export]Hint Resolve γ_ok_cons' Interp_back_preservation' : core.
-
-(* InterpUniv_RelProd_extdeter *)
-
-Definition SemWt' {n} (Γ : context n) a A : Prop :=
-  forall γ, γ_ok' γ Γ -> exists PA, Interp_rel A PA /\ PA (subst_tm γ a).
-
-
-Lemma Interp_Fun' A PA B (PB PF : tm 0 -> Prop) :
-  Interp_rel A PA ->
-  PF = (Prod PA PB) ->
-  Interp_rel B PB ->
-  Interp_rel (Fun A B) PF.
-Proof. hauto lq:on ctrs:Interp_rel. Qed.
-
-Lemma Interp_deterministic A PA PB : Interp_rel A PA -> Interp_rel A PB -> PA = PB.
-Proof.
-  elim : A PA PB.
-  - move => A hA B hB PA PB hPA hPB.
-    inversion hPA; subst.
-    inversion hPB; subst.
-    rewrite /Prod.
-    fext.
-    move => a b.
-    apply propositional_extensionality.
-    split.
-    + move => hA0 hb.
-      have ? : PA = PA0 by sfirstorder.
-      subst.
-      have ? : PB1 = PB0 by sfirstorder.
-      subst.
-      sfirstorder.
-    + move => hA0 hb.
-      have ? : PA = PA0 by sfirstorder.
-      have ? : PB1 = PB0 by sfirstorder.
-      sfirstorder.
-  - hauto lq:on inv:Interp_rel.
-Qed.
-
-Lemma fundamental_lemma' {n} (Γ : context n) a A (h : Wt Γ a A) :
-  SemWt' Γ a A.
-Proof.
-    elim : n Γ a A /h; rewrite /SemWt'.
-    - sfirstorder.
-    - move => n Γ A a B h0 ih0 γ hγ.
-      (* The well-formedness condition would have given me the admitted fact *)
-      have [PA hA] : exists PA, Interp_rel A PA by admit.
-      exists (Prod PA (fun a => exists K, Interp_rel B K /\ K a)).
-      split.
-      + constructor; auto.
-        move => a0 ha0.
-        case /(_ (a0 .: γ) ltac:(eauto)) : ih0 => PB [h1 h2].
-        suff : (fun a1 : tm 0 => exists K : tm 0 -> Prop, Interp_rel B K /\ K a1) =
-                 PB by congruence.
-        fext.
-        move => b.
-        apply propositional_extensionality.
-        split; last by sfirstorder.
-        move => [K [h3 h4]].
-        suff : K = PB by congruence.
-        sfirstorder use:Interp_deterministic.
-      + rewrite /Prod.
-        move => b hb.
-        move /(_ (b .: γ) ltac:(eauto)) in ih0.
-        case : ih0 => K' [h1 h2].
-        exists K'.
-        split; simpl; auto.
-        apply : Interp_rel_back_preservation; eauto.
-        by asimpl.
+  elim : A n a h.
+  - move => /= A ihA B ihB n a ha.
 Admitted.
